Modify the definition of atomic_body

examples/elimination_stack/StackA.v
@@ -2,7 +2,7 @@ Require Import CRIS.
 Require Import MemHeader MemA.
 Require Import SchHeader SchA.
 From CRIS.helping Require Import Header HelpingTactics.
-Require Import StackHeader.
+Require Import StackHeader IndefiniteDescription.
 
 Class stackG (jobID retID : Type) `{!crisG Γ Σ α β τ _S _I} := StackG {
   stack_tokG :: inG (exclR unitO) Γ;
@@ -150,8 +150,7 @@ Section definitions.
          (λ ret, True))))%I.
 End definitions.
 
-(* TODO : come back when you define atomic_body *)
-(* Module StackM. Section StackM.
+Module StackM. Section StackM.
   Definition jobID : Type := nat * nat * (nat * val * val * gname).
   Definition retID : Type := val.
 
@@ -161,7 +160,7 @@ End definitions.
   (* Module definitions *)
   Definition scopes : gmultiset string := ∅.
 
-  Definition jobCode : jobID → itree Helping.pureE retID :=
+  Definition jobCode : jobID → itree crisE retID :=
     λ '(_, _, (_, _, v, γs)),
       l <- trigger (Take (list (leibnizO val)));;
       trigger (Assume (stack_content γs l));;;
@@ -172,34 +171,33 @@ End definitions.
     λ _, 𝒴;;; trigger (Choose val).
 
   Definition push : Any.t → itree crisE Any.t :=
-    atomic_body (from_fspec (push_spec N)) (λ x arg, trigger (Call (Helping.run mn) x↑)).
+    atomic_body (push_spec N) (λ x _, trigger (Call (Helping.run mn) x↑)).
 
   Definition pop : Any.t → itree crisE Any.t :=
-    atomic_body (from_fspec (pop_spec N))
+    atomic_body (pop_spec N)
       (λ x _,
-        𝒴;;;
         'b : _ <- trigger (Choose bool);;
         (if b : bool then trigger (Call (Helping.help mn) ()↑) else Ret ()↑);;;
         l <- trigger (Take (list (leibnizO val)));;
         trigger (Assume (stack_content x.2.2 l));;;
         trigger (Guarantee (stack_content x.2.2 (tail l)));;;
         let vret := match l with | v :: _ => v | _ => Vundef end in
-        𝒴;;; Ret (vret↑)).
+        Ret (vret↑)).
 
-  Definition fnsems : fnsems_type :=
-    [(Some StackHdr.new_stack, (true, wmask_all, scopes, (Some (new_stack_spec N), cfunU new_stack)));
-     (Some StackHdr.push,      (true, wmask_all, scopes, (None, push)));
-     (Some StackHdr.pop,       (true, wmask_all, scopes, (None, pop)))].
+  Definition fnsems : fnsemmap :=
+    {[Some StackHdr.new_stack :=
+        Some (msk_scp scopes msk_true, (fsp_some (new_stack_spec N), cfunU new_stack));
+      Some StackHdr.push := Some (msk_scp scopes msk_true, (None, push));
+      Some StackHdr.push := Some (msk_scp scopes msk_true, (None, pop))]}.
 
   Program Definition Mod : SMod.t := {|
     SMod.scopes := scopes;
     SMod.fnsems := fnsems;
-    SMod.initial_st := [];
+    SMod.initial_st := ∅;
   |}.
-  Solve All Obligations with prove_scope.
-  Next Obligation. prove_nodup. Qed.
+  Solve All Obligations with mod_tac.
 
-  Definition t sp := Seal.sealing CRIS (SMod.to_mod sp Mod).
+  Definition t sp := SMod.to_mod sp Mod.
 End StackM. End StackM.
 
 Module StackA. Section StackA.
@@ -207,43 +205,40 @@ Module StackA. Section StackA.
   Context (N : namespace).
 
   (* Module definitions *)
-  Definition scopes : list string := [].
+  Definition scopes : gmultiset string := ∅.
 
   Definition new_stack : list val → itree crisE val :=
     λ _, 𝒴;;; trigger (Choose val).
 
   Definition push : Any.t → itree crisE Any.t :=
-    atomic_body (from_fspec (push_spec N))
+    atomic_body (push_spec N)
       (λ '(_, _, (_, _, v, γs)) _,
-        𝒴;;;
         l <- trigger (Take (list (leibnizO val)));;
         trigger (Assume (stack_content γs l));;;
         trigger (Guarantee (stack_content γs (v :: l)));;;
-        𝒴;;;
         Ret Vundef↑).
 
   Definition pop : Any.t → itree crisE Any.t :=
-    atomic_body (from_fspec (pop_spec N))
-      (λ '(_, _, (_, γs)) _,
-        𝒴;;;
+    atomic_body (pop_spec N)
+      (λ '(_, _, (_, γs)) _, 
         l <- trigger (Take (list (leibnizO val)));;
         trigger (Assume (stack_content γs l));;;
         trigger (Guarantee (stack_content γs (tail l)));;;
         let vret := match l with | v :: _ => v | _ => Vundef end in
-        𝒴;;; Ret (vret↑)).
+        Ret (vret↑)).
 
-  Definition fnsems : fnsems_type :=
-    [(Some StackHdr.new_stack, (true, wmask_all, scopes, (Some (new_stack_spec N), cfunU new_stack)));
-     (Some StackHdr.push,      (true, wmask_all, scopes, (None, push)));
-     (Some StackHdr.pop,       (true, wmask_all, scopes, (None, pop)))].
+  Definition fnsems : fnsemmap :=
+    {[Some StackHdr.new_stack :=
+        Some (msk_scp scopes msk_true, (fsp_some (new_stack_spec N), cfunU new_stack));
+      Some StackHdr.push := Some (msk_scp scopes msk_true, (None, push));
+      Some StackHdr.push := Some (msk_scp scopes msk_true, (None, pop))]}.
 
   Program Definition Mod : SMod.t := {|
     SMod.scopes := scopes;
     SMod.fnsems := fnsems;
-    SMod.initial_st := [];
+    SMod.initial_st := ∅;
   |}.
-  Solve All Obligations with prove_scope.
-  Next Obligation. prove_nodup. Qed.
+  Solve All Obligations with mod_tac.
 
-  Definition t sp := Seal.sealing CRIS (SMod.to_mod sp Mod).
-End StackA. End StackA. *)
+  Definition t sp := SMod.to_mod sp Mod.
+End StackA. End StackA.
